Update.

src/metalogic/fol/fol.lean
@@ -19,100 +19,100 @@ def is_repl_of_var_in_list_fun (u v : variable_) : list variable_ → list varia
 | _ _ := false
 
 
-def is_repl_of_var_fun (u v : variable_) : formula → formula → Prop
+def is_repl_of_var_in_formula_fun (u v : variable_) : formula → formula → Prop
 | true_ true_ := true
 | (pred_ name_u args_u) (pred_ name_v args_v) := name_u = name_v ∧ is_repl_of_var_in_list_fun u v args_u args_v
 | (eq_ x_u y_u) (eq_ x_v y_v) := (x_u = x_v ∨ (x_u = u ∧ x_v = v)) ∧ (y_u = y_v ∨ (y_u = u ∧ y_v = v))
-| (not_ P_u) (not_ P_v) := is_repl_of_var_fun P_u P_v
-| (imp_ P_u Q_u) (imp_ P_v Q_v) := is_repl_of_var_fun P_u P_v ∧ is_repl_of_var_fun Q_u Q_v
-| (forall_ x P_u) (forall_ x' P_v) := x = x' ∧ is_repl_of_var_fun P_u P_v
+| (not_ P_u) (not_ P_v) := is_repl_of_var_in_formula_fun P_u P_v
+| (imp_ P_u Q_u) (imp_ P_v Q_v) := is_repl_of_var_in_formula_fun P_u P_v ∧ is_repl_of_var_in_formula_fun Q_u Q_v
+| (forall_ x P_u) (forall_ x' P_v) := x = x' ∧ is_repl_of_var_in_formula_fun P_u P_v
 | _ _ := false
 
 
 /--
-is_repl_of_var u v P_u P_v = True if and only if P_v is the result of replacing one or more specified occurrences (but not necessarily all occurrences) of u in P_u by occurrences of v.
+is_repl_of_var_in_formula u v P_u P_v = True if and only if P_v is the result of replacing one or more specified occurrences (but not necessarily all occurrences) of u in P_u by occurrences of v.
 -/
-inductive is_repl_of_var (u v : variable_) : formula → formula → Prop
+inductive is_repl_of_var_in_formula (u v : variable_) : formula → formula → Prop
 | true_ :
-  is_repl_of_var true_ true_
+  is_repl_of_var_in_formula true_ true_
 
 | pred_
   (name : pred_name_)
   (n : ℕ)
   (args_u args_v : fin n → variable_) :
   (∀ (i : fin n), (args_u i = args_v i) ∨ (args_u i = u ∧ args_v i = v)) →
-  is_repl_of_var (pred_ name (list.of_fn args_u)) (pred_ name (list.of_fn args_v))
+  is_repl_of_var_in_formula (pred_ name (list.of_fn args_u)) (pred_ name (list.of_fn args_v))
 
 | eq_
   (x_u y_u : variable_)
   (x_v y_v : variable_) :
   (x_u = x_v) ∨ (x_u = u ∧ x_v = v) →
   (y_u = y_v) ∨ (y_u = u ∧ y_v = v) →
-  is_repl_of_var (eq_ x_u y_u) (eq_ x_v y_v)
+  is_repl_of_var_in_formula (eq_ x_u y_u) (eq_ x_v y_v)
 
 | not_
   (P_u P_v : formula) :
-  is_repl_of_var P_u P_v →
-  is_repl_of_var P_u.not_ P_v.not_
+  is_repl_of_var_in_formula P_u P_v →
+  is_repl_of_var_in_formula P_u.not_ P_v.not_
 
 | imp_
   (P_u Q_u : formula)
   (P_v Q_v : formula) :
-  is_repl_of_var P_u P_v →
-  is_repl_of_var Q_u Q_v →
-  is_repl_of_var (P_u.imp_ Q_u) (P_v.imp_ Q_v)
+  is_repl_of_var_in_formula P_u P_v →
+  is_repl_of_var_in_formula Q_u Q_v →
+  is_repl_of_var_in_formula (P_u.imp_ Q_u) (P_v.imp_ Q_v)
 
 | forall_
   (x : variable_)
   (P_u P_v : formula) :
-  is_repl_of_var P_u P_v →
-  is_repl_of_var (forall_ x P_u) (forall_ x P_v)
+  is_repl_of_var_in_formula P_u P_v →
+  is_repl_of_var_in_formula (forall_ x P_u) (forall_ x P_v)
 
 
 /--
-is_repl_of_formula_fun U V P_u P_v = True if and only if P_v is the result of replacing one or more specified occurrences (but not necessarily all occurrences) of U in P_u by occurrences of V.
+is_repl_of_formula_in_formula_fun U V P_u P_v = True if and only if P_v is the result of replacing one or more specified occurrences (but not necessarily all occurrences) of U in P_u by occurrences of V.
 -/
-def is_repl_of_formula_fun (U V : formula) : formula → formula → Prop
-| (not_ P_u) (not_ P_v) := is_repl_of_formula_fun P_u P_v
-| (imp_ P_u Q_u) (imp_ P_v Q_v) := is_repl_of_formula_fun P_u P_v ∧ is_repl_of_formula_fun Q_u Q_v
-| (forall_ x P_u) (forall_ x' P_v) := x = x' ∧ is_repl_of_formula_fun P_u P_v
+def is_repl_of_formula_in_formula_fun (U V : formula) : formula → formula → Prop
+| (not_ P_u) (not_ P_v) := is_repl_of_formula_in_formula_fun P_u P_v
+| (imp_ P_u Q_u) (imp_ P_v Q_v) := is_repl_of_formula_in_formula_fun P_u P_v ∧ is_repl_of_formula_in_formula_fun Q_u Q_v
+| (forall_ x P_u) (forall_ x' P_v) := x = x' ∧ is_repl_of_formula_in_formula_fun P_u P_v
 | P_u P_v := P_u = P_v ∨ (P_u = U ∧ P_v = V)
 
 
 /--
-is_repl_of_formula U V P_u P_v = True if and only if P_v is the result of replacing one or more specified occurrences (but not necessarily all occurrences) of U in P_u by occurrences of V.
+is_repl_of_formula_in_formula U V P_u P_v = True if and only if P_v is the result of replacing one or more specified occurrences (but not necessarily all occurrences) of U in P_u by occurrences of V.
 -/
-inductive is_repl_of_formula (U V : formula) : formula → formula → Prop
+inductive is_repl_of_formula_in_formula (U V : formula) : formula → formula → Prop
 -- not replacing an occurrence
 | same_
   (P_u P_v : formula) :
   P_u = P_v →
-  is_repl_of_formula P_u P_v
+  is_repl_of_formula_in_formula P_u P_v
 
 -- replacing an occurrence
 | diff_
   (P_u P_v : formula) :
   P_u = U →
   P_v = V →
-  is_repl_of_formula P_u P_v
+  is_repl_of_formula_in_formula P_u P_v
 
 | not_
   (P_u P_v : formula) :
-  is_repl_of_formula P_u P_v →
-  is_repl_of_formula P_u.not_ P_v.not_
+  is_repl_of_formula_in_formula P_u P_v →
+  is_repl_of_formula_in_formula P_u.not_ P_v.not_
 
 | imp_
   (P_u Q_u : formula)
   (P_v Q_v : formula) :
-  is_repl_of_formula P_u P_v →
-  is_repl_of_formula Q_u Q_v →
-  is_repl_of_formula (P_u.imp_ Q_u) (P_v.imp_ Q_v)
+  is_repl_of_formula_in_formula P_u P_v →
+  is_repl_of_formula_in_formula Q_u Q_v →
+  is_repl_of_formula_in_formula (P_u.imp_ Q_u) (P_v.imp_ Q_v)
 
 | forall_
   (x : variable_)
   (P_u P_v : formula) :
-  is_repl_of_formula P_u P_v →
-  is_repl_of_formula (forall_ x P_u) (forall_ x P_v)
+  is_repl_of_formula_in_formula P_u P_v →
+  is_repl_of_formula_in_formula (forall_ x P_u) (forall_ x P_v)
 
 
 def similar (P_u P_v : formula) (u v : variable_) : Prop :=
@@ -976,25 +976,25 @@ theorem T_18_2
   (U V : formula)
   (P_U P_V : formula)
   (l : list variable_)
-  (h1 : is_repl_of_formula U V P_U P_V)
+  (h1 : is_repl_of_formula_in_formula U V P_U P_V)
   (h2 : ∀ (v : variable_), ((is_free_in v U ∨ is_free_in v V) ∧ is_bound_in v P_U) → v ∈ l) :
   is_proof ((Forall_ l (U.iff_ V)).imp_ (P_U.iff_ P_V)) :=
 begin
   induction h1,
-  case is_repl_of_formula.same_ : h1_P h1_P' h1_1
+  case is_repl_of_formula_in_formula.same_ : h1_P h1_P' h1_1
   {
     subst h1_1,
     apply deduction_theorem,
     apply proof_imp_deduct,
     apply prop_iff_id,
   },
-  case is_repl_of_formula.diff_ : h1_P h1_P' h1_1 h1_2
+  case is_repl_of_formula_in_formula.diff_ : h1_P h1_P' h1_1 h1_2
   {
     subst h1_1,
     subst h1_2,
     apply Forall_spec_id,
   },
-  case is_repl_of_formula.not_ : h1_P h1_P' h1_1 h1_ih
+  case is_repl_of_formula_in_formula.not_ : h1_P h1_P' h1_1 h1_ih
   {
     unfold is_bound_in at h2,
 
@@ -1011,7 +1011,7 @@ begin
       exact h1_ih h2,
     },
   },
-  case is_repl_of_formula.imp_ : h1_P h1_Q h1_P' h1_Q' h1_1 h1_2 h1_ih_1 h1_ih_2
+  case is_repl_of_formula_in_formula.imp_ : h1_P h1_Q h1_P' h1_Q' h1_1 h1_2 h1_ih_1 h1_ih_2
   {
     unfold is_bound_in at h2,
 
@@ -1040,7 +1040,7 @@ begin
       tauto,
     },
   },
-  case is_repl_of_formula.forall_ : h1_x h1_P h1_P' h1_1 h1_ih
+  case is_repl_of_formula_in_formula.forall_ : h1_x h1_P h1_P' h1_1 h1_ih
   {
     unfold is_bound_in at h2,
 
@@ -1091,7 +1091,7 @@ end
 theorem C_18_3
   (U V : formula)
   (P_U P_V : formula)
-  (h1 : is_repl_of_formula U V P_U P_V)
+  (h1 : is_repl_of_formula_in_formula U V P_U P_V)
   (h2 : is_proof (U.iff_ V)) :
   is_proof (P_U.iff_ P_V) :=
 begin
@@ -1131,7 +1131,7 @@ theorem C_18_4
   (U V : formula)
   (P_U P_V : formula)
   (Δ : set formula)
-  (h1 : is_repl_of_formula U V P_U P_V)
+  (h1 : is_repl_of_formula_in_formula U V P_U P_V)
   (h2 : is_proof (U.iff_ V))
   (h3 : is_deduct Δ P_U) :
   is_deduct Δ P_V :=
@@ -1246,7 +1246,7 @@ theorem T_18_7
   (u v : variable_)
   (Δ : set formula)
   (h1 : is_deduct Δ Q)
-  (h2 : is_repl_of_formula (forall_ u P_u) (forall_ v P_v) Q Q')
+  (h2 : is_repl_of_formula_in_formula (forall_ u P_u) (forall_ v P_v) Q Q')
   (h3 : similar P_u P_v u v) :
   is_deduct Δ Q' :=
 begin
@@ -1331,15 +1331,15 @@ theorem T_19_TS_21_left
 begin
   apply C_18_4 (forall_ v P) P ((forall_ v (P.imp_ Q)).imp_ ((forall_ v P).imp_ (forall_ v Q))),
   {
-    apply is_repl_of_formula.imp_,
+    apply is_repl_of_formula_in_formula.imp_,
     {
-      apply is_repl_of_formula.same_,
+      apply is_repl_of_formula_in_formula.same_,
       refl,
     },
     {
-      apply is_repl_of_formula.imp_,
+      apply is_repl_of_formula_in_formula.imp_,
       {
-        apply is_repl_of_formula.diff_,
+        apply is_repl_of_formula_in_formula.diff_,
         {
           refl,
         },
@@ -1348,7 +1348,7 @@ begin
         },
       },
       {
-        apply is_repl_of_formula.same_,
+        apply is_repl_of_formula_in_formula.same_,
         refl,
       },
     }
@@ -1522,26 +1522,26 @@ end
 theorem T_21_8
   (P_r P_s : formula)
   (r s : variable_)
-  (h1 : is_repl_of_var r s P_r P_s)
+  (h1 : is_repl_of_var_in_formula r s P_r P_s)
   (h2 : occurs_in r P_r)
   (h3 : ¬ is_bound_in r P_r)
   (h4 : ¬ is_bound_in s P_r) :
   is_proof ((eq_ r s).imp_ (P_r.iff_ P_s)) :=
 begin
   induction h1,
-  case is_repl_of_var.true_
+  case is_repl_of_var_in_formula.true_
   { admit },
-  case is_repl_of_var.pred_ : h1_name h1_n h1_args h1_args' h1_1
+  case is_repl_of_var_in_formula.pred_ : h1_name h1_n h1_args h1_args' h1_1
   {
     exact T_21_8_pred h1_name h1_n h1_args h1_args' r s h1_1,
   },
-  case is_repl_of_var.eq_ : h1_x h1_y h1_x' h1_y' h1_ᾰ h1_ᾰ_1
+  case is_repl_of_var_in_formula.eq_ : h1_x h1_y h1_x' h1_y' h1_ᾰ h1_ᾰ_1
   { admit },
-  case is_repl_of_var.not_ : h1_P h1_P' h1_ᾰ h1_ih
+  case is_repl_of_var_in_formula.not_ : h1_P h1_P' h1_ᾰ h1_ih
   { admit },
-  case is_repl_of_var.imp_ : h1_P h1_Q h1_P' h1_Q' h1_ᾰ h1_ᾰ_1 h1_ih_ᾰ h1_ih_ᾰ_1
+  case is_repl_of_var_in_formula.imp_ : h1_P h1_Q h1_P' h1_Q' h1_ᾰ h1_ᾰ_1 h1_ih_ᾰ h1_ih_ᾰ_1
   { admit },
-  case is_repl_of_var.forall_ : h1_x h1_P h1_P' h1_1 h1_ih
+  case is_repl_of_var_in_formula.forall_ : h1_x h1_P h1_P' h1_1 h1_ih
   {
     unfold occurs_in at h2,
 
